Lib.v
@@ -737,6 +737,25 @@ Proof.
   by invert; apply ord_inj.
 Qed.
 
+Lemma widen_ord_spec : forall n x (H : n <= n), widen_ord H x = x.
+Proof.
+  move=> ? [? ?] ?.
+  rewrite /widen_ord.
+  congr (Ordinal _).
+  exact: eq_irrelevance.
+Qed.
+
+Lemma widen_fst_inj : forall a n, injective (@widen_fst n a).
+Proof.
+  move=> a n.
+  rewrite /injective => [[[x1a H1] x1b] [[x2a H2] x2b]].
+  invert.
+  congr (_, _).
+  rewrite H0 in H1 *.
+  congr (Ordinal _).
+  exact: eq_irrelevance.
+Qed.
+
 Lemma no_ord_max : forall n (xs : seq ('I_n)),
   ord_max \notin [ seq widen_id i | i <- xs ].
 Proof.
